SPos/Semantics/Type.lean
@@ -2,6 +2,8 @@ import SPos.Structure.PER
 import SPos.Semantics.DomainTheory.Domain
 import SPos.Semantics.ValueDomain
 
+open ScottDomain
+
 variable
   {D : Type u} [ScottDomain D Label]
 
@@ -26,6 +28,38 @@ def PER.pi (dom : PER D) (cod : dom →ₚ PER.diag (PER D)) : PER D where
     exact hgh y y hyy
   ⟩
 
+
+def PER.sigma (dom : PER D) (cod : dom →ₚ PER.diag (PER D)) : PER D where
+  rel p q := ∃ a b a' b', p = mkPair a b ∧ q = mkPair a' b'
+              ∧ (a ~ a' ∈ₚ dom) ∧ (b ~ b' ∈ₚ cod a)
+
+  sym := ⟨ fun p q h => by
+    obtain ⟨a, b, a', b', rfl, rfl, h₁, h₂⟩ := h
+    have hcod : cod a = cod a' := cod.respRelation _ _ h₁
+    exact ⟨a', b', a, b, rfl, rfl, PER.symm _ h₁, hcod ▸ PER.symm _ h₂⟩
+  ⟩
+
+  tra := ⟨ fun p q r hpq hqr => by
+    obtain ⟨a, b, a', b', rfl, hq, h₁, h₂⟩ := hpq
+    obtain ⟨a'', b'', a₃, b₃, hq', rfl, h₃, h₄⟩ := hqr
+    obtain ⟨rfl, rfl⟩ := mkPair_inj (hq.symm.trans hq')
+    have hcod : cod a = cod a' := cod.respRelation _ _ h₁
+    exact ⟨a, b, a₃, b₃, rfl, rfl, PER.trans _ h₁ h₃, PER.trans _ h₂ (hcod ▸ h₄)⟩
+  ⟩
+
+def PER.bool : PER D where
+  rel u v := (u = mkTrue ∧ v = mkTrue) ∨ (u = mkFalse ∧ v = mkFalse)
+  sym := ⟨ fun u v h => by rcases h with ⟨rfl, rfl⟩ | ⟨rfl, rfl⟩ <;> simp ⟩
+  tra := ⟨ fun u v w huv hvw => by
+    rcases huv with ⟨rfl, rfl⟩ | ⟨rfl, rfl⟩
+    · rcases hvw with ⟨_, rfl⟩ | ⟨hv, _⟩
+      · exact Or.inl ⟨rfl, rfl⟩
+      · exact absurd hv mkTrue_ne_mkFalse
+    · rcases hvw with ⟨hv, _⟩ | ⟨_, rfl⟩
+      · exact absurd hv.symm mkTrue_ne_mkFalse
+      · exact Or.inr ⟨rfl, rfl⟩
+  ⟩
+
 def PER.id (A : PER D) (a b : D) : PER D where
   rel _ _ := a ~ b ∈ₚ A
   sym := ⟨ fun _ _ h => h ⟩
@@ -35,5 +69,6 @@ omit [ScottDomain D Label] in
 theorem PER.id_congr (ha : a ~ a' ∈ₚ A) (hb : b ~ b' ∈ₚ A) :
     PER.id A a b = PER.id A a' b' := by
   apply PER.ext; funext x y; apply propext
-  exact ⟨fun h => A.trans (A.trans (A.symm ha) h) hb,
-         fun h => A.trans (A.trans ha h) (A.symm hb)⟩
+  grind [PER.id, PER.diag, PER.symm, PER.trans]
+  -- exact ⟨fun h => A.trans (A.trans (A.symm ha) h) hb,
+  --        fun h => A.trans (A.trans ha h) (A.symm hb)⟩
