SPos.lean
@@ -9,6 +9,7 @@ import SPos.Semantics.ValueDomain
 import SPos.Structure.PER
 import SPos.Syntax.Syntax
 import SPos.Syntax.SyntaxProperties
+import SPos.Typing.DerivedSum
 import SPos.Typing.Regularity
 import SPos.Typing.Sound
 import SPos.Typing.Substitution
